\documentclass[11pt,a4paper]{article}
\usepackage[utf8]{inputenc}
\usepackage{amsmath}
\usepackage{amsfonts}
\usepackage{amssymb}
\usepackage{xcolor}
\usepackage{array,booktabs}
\usepackage[none]{hyphenat}
\usepackage{geometry}
\usepackage{graphicx}
\geometry{margin=2.5cm}
\usepackage{float}
\usepackage{multirow}
\usepackage{amsthm}
\usepackage{hyperref}
\theoremstyle{plain}
\newtheorem{thm}{Theorem}[section] % reset theorem numbering for each chapter

\theoremstyle{definition}
\newtheorem{defn}[thm]{Definition} % definition numbers are dependent on theorem numbers
\newtheorem{exmp}[thm]{Example} % same for example numbers
%\usepackage{cmbright}
\usepackage{fancyhdr}
\pagestyle{fancy}
\fancyhf{}
\rhead{Biharmonic Tests}
\lhead{\leftmark}
\rfoot{\thepage}
\author{}
\title{}
\begin{document}
\tableofcontents
\listoftables

\dotfill
\section{01-01 tests}
\begin{exmp}
\label{Example:PRO:bending:01_01_glob3}
In this tests we consider:
\begin{itemize}
\item $\psi(x)=x^4$
\item $\psi_\text l=0$
\item $\psi_\text r=1$
\item $\psi_\text{ll}=0$
\item $\psi_\text{rr}=4$
\item $g(x)=-24$
\end{itemize}
\end{exmp}
\input{../table_01_01_glob3.tex}
%\input{../test_01_01_test9/output/test_01_01_test9.tex}
%\input{../test_01_01_test10/output/test_01_01_test10.tex}
%\input{../test_01_01_test11/output/test_01_01_test11.tex}
%\input{../test_01_01_test12/output/test_01_01_test12.tex}

\pagebreak

\begin{exmp}
\label{Example:PRO:bending:01_01_glob1}
In this tests we consider:
\begin{itemize}
\item $\psi(x)=\exp(x)$
\item $\psi_\text l=1$
\item $\psi_\text r=e$
\item $\psi_\text{ll}=1$
\item $\psi_\text{rr}=e$
\item $g(x)=-\exp(x)$
\end{itemize}
\end{exmp}
\input{../table_01_01_glob1.tex}
\input{../table_01_01_glob1_full_weights.tex}
%\input{../test_01_01_test1/output/test_01_01_test1.tex}
%\input{../test_01_01_test2/output/test_01_01_test2.tex}
%\input{../test_01_01_test3/output/test_01_01_test3.tex}
%\input{../test_01_01_test4/output/test_01_01_test4.tex}
\pagebreak 

%\begin{exmp}
%\label{Example:PRO:bending:01_01_glob4}
%In this tests we consider:
%\begin{itemize}
%\item $\psi(x)=\exp(x)$
%\item $\psi_\text l=1$
%\item $\psi_\text r=e$
%\item $\psi_\text{ll}=1$
%\item $\psi_\text{rr}=e$
%\item $g(x)=-\exp(x)$
%\end{itemize}
%\end{exmp}
%\input{../table_01_01_glob4.tex}
%%\input{../test_01_01_test13/output/test_01_01_test13.tex}
%%\input{../test_01_01_test14/output/test_01_01_test14.tex}
%%\input{../test_01_01_test15/output/test_01_01_test15.tex}
%%\input{../test_01_01_test16/output/test_01_01_test16.tex}

%\pagebreak
\begin{exmp}
\label{Example:PRO:bending:01_01_glob2}
In this tests we consider:
\begin{itemize}
\item $\psi(x)=-\exp(x)+x^3(3-e)+x^2(2e-5)+x+1$
\item $\psi_\text l=0$
\item $\psi_\text r=0$
\item $\psi_\text{ll}=0$
\item $\psi_\text{rr}=0$
\item $g(x)=\exp(x)$
\end{itemize}
\end{exmp}
\input{../table_01_01_glob2.tex}
%\input{../test_01_01_test5/output/test_01_01_test5.tex}
%\input{../test_01_01_test6/output/test_01_01_test6.tex}
%\input{../test_01_01_test7/output/test_01_01_test7.tex}
%\input{../test_01_01_test8/output/test_01_01_test8.tex}

\pagebreak

%%%%%%%%%%%%%%%%%%%%%%%%%%%%%%%%%%%%%%%%%%%%%%%%%%%%%%%%%%%%%
\section{02-02 tests}

\begin{exmp}
\label{Example:PRO:bending:02_02_glob3}
In this tests we consider:
\begin{itemize}
\item $\psi(x)=x^4$
\item $\psi_\text l=0$
\item $\psi_\text r=1$
\item $M_\text l=0$
\item $M_\text r=-12$
\item $g(x)=-24$
\end{itemize}
\end{exmp}
\input{../table_02_02_glob3.tex}
%\input{../test_02_02_test9/output/test_02_02_test9.tex}
%\input{../test_02_02_test10/output/test_02_02_test10.tex}
%\input{../test_02_02_test11/output/test_02_02_test11.tex}
%\input{../test_02_02_test12/output/test_02_02_test12.tex}
\pagebreak

\begin{exmp}
\label{Example:PRO:bending:02_02_glob6}
In this tests we consider:
\begin{itemize}
\item $\psi(x)=\exp(x)$
\item $\psi_\text l=1$
\item $\psi_\text r=e$
\item $M_\text l=-1$
\item $M_\text r=-e$
\item $g(x)=-\exp(x)$
\end{itemize}
\end{exmp}
\input{../table_02_02_glob6.tex}
\pagebreak
%\input{../test_02_02_test21/output/test_02_02_test21.tex}
%\input{../test_02_02_test22/output/test_02_02_test22.tex}
%\input{../test_02_02_test23/output/test_02_02_test23.tex}
%\input{../test_02_02_test24/output/test_02_02_test24.tex}
%\pagebreak

%\begin{exmp}
%\label{Example:PRO:bending:02_02_glob1}
%In this tests we consider:
%\begin{itemize}
%\item $\psi(x)=-\frac{x^4}{24}+\frac{x^3}{12}-\frac{x}{24}$
%\item $\psi_\text l=0$
%\item $\psi_\text r=0$
%\item $M_\text l=0$
%\item $M_\text r=0$
%\item $g(x)=1$
%\end{itemize}
%\end{exmp}
%\input{../table_02_02_glob1.tex}
%\input{../test_02_02_test1/output/test_02_02_test1.tex}
%\input{../test_02_02_test2/output/test_02_02_test2.tex}
%\input{../test_02_02_test3/output/test_02_02_test3.tex}
%\input{../test_02_02_test4/output/test_02_02_test4.tex}
%\pagebreak

\begin{exmp}
\label{Example:PRO:bending:02_02_glob2}
In this tests we consider:
\begin{itemize}
\item $\psi(x)=-\exp(x)+\left(\frac{e-1}{6}\right)x^3+\frac{x^2}{2}+\left(\frac{5e-8}{6}\right)x+1$
\item $\psi_\text l=0$
\item $\psi_\text r=0$
\item $M_\text l=0$
\item $M_\text r=0$
\item $g(x)=\exp(x)$
\end{itemize}
\end{exmp}
\input{../table_02_02_glob2.tex}
%\input{../test_02_02_test5/output/test_02_02_test5.tex}
%\input{../test_02_02_test6/output/test_02_02_test6.tex}
%\input{../test_02_02_test7/output/test_02_02_test7.tex}
%\input{../test_02_02_test8/output/test_02_02_test8.tex}
\pagebreak

%\begin{exmp}
%\label{Example:PRO:bending:02_02_glob4}
%In this tests we consider:
%\begin{itemize}
%\item $\psi(x)=-\exp(x)+x^3\left(\frac{\text e-1}{6}\right)+x^2+x\left(\frac{5\text e-11}{6}\right)+1$
%\item $\psi_\text l=0$
%\item $\psi_\text r=1$
%\item $M_\text l=1$
%\item $M_\text r=1$
%\item $g(x)=\exp(x)$
%\end{itemize}
%\end{exmp}
%\input{../table_02_02_glob4.tex}
%%\input{../test_02_02_test13/output/test_02_02_test13.tex}
%%\input{../test_02_02_test14/output/test_02_02_test14.tex}
%%\input{../test_02_02_test15/output/test_02_02_test15.tex}
%%\input{../test_02_02_test16/output/test_02_02_test16.tex}
%\pagebreak

%\begin{exmp}
%\label{Example:PRO:bending:02_02_glob5}
%In this tests we consider:
%\begin{itemize}
%\item $\psi(x)=-\exp(x)+x^3\left(\frac{\text e-1}{6}\right)+x\left(\frac{11\text e-11}{6}\right)+2$
%\item $\psi_\text l=1$
%\item $\psi_\text r=e$
%\item $M_\text l=1$
%\item $M_\text r=1$
%\item $g(x)=\exp(x)$
%\end{itemize}
%\end{exmp}
%\input{../table_02_02_glob5.tex}
%%\input{../test_02_02_test17/output/test_02_02_test17.tex}
%%\input{../test_02_02_test18/output/test_02_02_test18.tex}
%%\input{../test_02_02_test19/output/test_02_02_test19.tex}
%%\input{../test_02_02_test20/output/test_02_02_test20.tex}
%\pagebreak


%%%%%%%%%%%%%%%%%%%%%%%%%%%%%%%%%%%%%%%%%%%%%%%%%%%%%%%%%%%%%
\section{01-23 tests}

\begin{exmp}
\label{Example:PRO:bending:01_23_glob3}
In this tests we consider:
\begin{itemize}
\item $\psi(x)=x^4$
\item $\psi_\text l=0$
\item $\psi_\text{ll}=0$
\item $M_\text r=-12$
\item $G=-24$
\item $g(x)=24$
\end{itemize}
\end{exmp}
\input{../table_01_23_glob3.tex}
%\input{../test_01_23_test9/output/test_01_23_test9.tex}
%\input{../test_01_23_test10/output/test_01_23_test10.tex}
%\input{../test_01_23_test11/output/test_01_23_test11.tex}
%\input{../test_01_23_test12/output/test_01_23_test12.tex}
\pagebreak

\begin{exmp}
\label{Example:PRO:bending:01_23_glob1}
In this tests we consider:
\begin{itemize}
\item $\psi(x)=\exp(x)$
\item $\psi_\text l=1$
\item $\psi_\text{ll}=1$
\item $M_\text r=-\text e$
\item $G=-\text e$
\item $g(x)=-\exp(x)$
\end{itemize}
\end{exmp}
\input{../table_01_23_glob1.tex}

%\input{../test_01_23_test1/output/test_01_23_test1.tex}
%\input{../test_01_23_test2/output/test_01_23_test2.tex}
%\input{../test_01_23_test3/output/test_01_23_test3.tex}
%\input{../test_01_23_test4/output/test_01_23_test4.tex}
\pagebreak

%\begin{exmp}
%\label{Example:PRO:bending:01_23_glob5}
%In this tests we consider:
%\begin{itemize}
%\item $\psi(x)=\exp(x)$
%\item $\psi_\text l=1$
%\item $\psi_\text{ll}=1$
%\item $M_\text r=-\text e$
%\item $G=-\text e$
%\item $g(x)=-\exp(x)$
%\end{itemize}
%\end{exmp}
%\input{../table_01_23_glob5.tex}
%%\input{../test_01_23_test17/output/test_01_23_test17.tex}
%%\input{../test_01_23_test18/output/test_01_23_test18.tex}
%%\input{../test_01_23_test19/output/test_01_23_test19.tex}
%%\input{../test_01_23_test20/output/test_01_23_test20.tex}
%\pagebreak

\begin{exmp}
\label{Example:PRO:bending:01_23_glob2}
In this tests we consider:
\begin{itemize}
\item $\psi(x)=-\exp(x)+x^3\left(\frac{\text e-1}{6}\right)+\frac{x^2}{2}+x+1$
\item $\psi_\text l=0$
\item $\psi_\text{ll}=0$
\item $M_\text r=0$
\item $G=1$
\item $g(x)=\exp(x)$
\end{itemize}
\end{exmp}
\input{../table_01_23_glob2.tex}
%\input{../test_01_23_test5/output/test_01_23_test5.tex}
%\input{../test_01_23_test6/output/test_01_23_test6.tex}
%\input{../test_01_23_test7/output/test_01_23_test7.tex}
%\input{../test_01_23_test8/output/test_01_23_test8.tex}
\pagebreak

%\begin{exmp}
%\label{Example:PRO:bending:01_23_glob4}
%In this tests we consider:
%\begin{itemize}
%\item $\psi(x)=-\exp(x)+x^3\left(\frac{\text e-1}{6}\right)+2x+2$
%\item $\psi_\text l=0$
%\item $\psi_\text{ll}=0$
%\item $M_\text r=0$
%\item $G=1$
%\item $g(x)=\exp(x)$
%\end{itemize}
%\end{exmp}
%\input{../table_01_23_glob4.tex}
%\input{../test_01_23_test13/output/test_01_23_test13.tex}
%\input{../test_01_23_test14/output/test_01_23_test14.tex}
%\input{../test_01_23_test15/output/test_01_23_test15.tex}
%\input{../test_01_23_test16/output/test_01_23_test16.tex}
\pagebreak


\end{document}
% end of file